logic.lean
@@ -2,83 +2,101 @@ import .syntax .notations .evaluation .substitution .qi
 
 -- validity
 
-inductive valid : vc → Prop
-notation `⊨` p: 100 := valid p
-
-| tru:
-  ⊨ value.true
-
-| unop {op: unop} {vₓ v: value}:
-  unop.apply op vₓ = some v →
-  ⊨ term.binop binop.eq (term.unop op vₓ) v
-
-| binop {op: binop} {v₁ v₂ v: value}:
-  binop.apply op v₁ v₂ = some v →
-  ⊨ term.binop binop.eq (term.binop op v₁ v₂) v
-
-| app {vₓ v: value} {σ σ': env} {f x y: var} {R S: spec} {e: exp}:
-  (σ[x↦vₓ], e) ⟶* (σ', exp.return y) →
-  (σ' y = some v) →
-  ⊨ term.binop binop.eq (term.app (value.func f x R S e σ) vₓ) v
-
-| and {P Q: vc}:
-  ⊨ P →
-  ⊨ Q →
-  ⊨ (P && Q)
-
-| orl {P Q: vc}:
-  ⊨ P →
-  ⊨ (P || Q)
-
-| orr {P Q: vc}:
-  ⊨ Q →
-  ⊨ (P || Q)
-
-| pre {vₓ: value} {σ: env} {f x y: var} {R S: spec} {e: exp}:
-  ⊨ vc.subst_env (σ[x↦vₓ][f↦value.func f x R S e σ]) R.to_prop.instantiated →
-  ⊨ vc.pre (value.func f x R S e σ) vₓ
-
-| pre₁ {vₓ v: value} {op: unop}:
-  (∃v, unop.apply op vₓ = some v) →
-  ⊨ vc.pre₁ op vₓ
-
-| pre₂ {v₁ v₂ v: value} {op: binop}:
-  (∃v, binop.apply op v₁ v₂ = v) →
-  ⊨ vc.pre₂ op v₁ v₂
-
-| post {vₓ: value} {σ σ': env} {f x y: var} {R S: spec} {e: exp}:
-  (σ[x↦vₓ], e) ⟶* (σ', exp.return y) →
-  ⊨ vc.subst_env (σ[x↦vₓ][f↦value.func f x R S e σ]) (spec.implies R S).to_prop.instantiated →
-  ⊨ vc.post (value.func f x R S e σ) vₓ
-
-| univ {x: var} {P: vc}:
-  (∀v, ⊨ vc.subst x v P) →
-  ⊨ vc.univ x P
-
+constant valid : vc → Prop
 notation `⊨` p: 100 := valid p
 notation σ `⊨` p: 100 := valid (vc.subst_env σ p)
-
-axiom valid.mp  {P Q: vc}: ⊨ vc.implies P Q → ⊨ P → ⊨ Q
-
-axiom valid.subst {t₁ t₂: term} (Q: propctx): ⊨ (t₁ ≡ t₂) → ⊨ (Q t₁).instantiated → ⊨ (Q t₂).instantiated
-
--- notation ⟪ P ⟫
-
 @[reducible]
 def VC(P: prop) := ∀ (σ: env), σ ⊨ P.instantiated
-
 notation `⟪` P `⟫`: 100 := VC P
 
-axiom instantiated_of_erased {σ: env} {P: prop}:
-  σ ⊨ P.erased → σ ⊨ P.instantiated
-axiom instantiated_n_of_instantiated {σ: env} {P: prop}:
-  σ ⊨ P.instantiated → σ ⊨ P.instantiated_n
-axiom erased_n_of_instantiated_n {σ: env} {P: prop}:
-  σ ⊨ P.instantiated_n → σ ⊨ P.erased_n
-axiom instantiated_and {σ: env} {P Q: prop}:
-  σ ⊨ P.instantiated → σ ⊨ Q.instantiated → σ ⊨ (P && Q).instantiated
-axiom instantiated_or {σ: env} {P Q: prop}:
-  σ ⊨ P.instantiated → σ ⊨ Q.instantiated → σ ⊨ (P || Q).instantiated
+-- axioms
+
+axiom valid.tru:
+  ⊨ value.true
+
+axiom valid.unop {op: unop} {vₓ v: value}:
+  unop.apply op vₓ = some v
+  ↔
+  ⊨ (term.unop op vₓ ≡ v)
+
+axiom valid.binop {op: binop} {v₁ v₂ v: value}:
+  binop.apply op v₁ v₂ = some v
+  ↔
+  ⊨ (term.binop op v₁ v₂ ≡ v)
+
+axiom valid.app {vₓ v: value} {σ σ': env} {f x y: var} {R S: spec} {e: exp}:
+  (σ[x↦vₓ], e) ⟶* (σ', exp.return y) ∧
+  (σ' y = some v)
+  ↔
+  ⊨ (term.app (value.func f x R S e σ) vₓ ≡ v)
+
+axiom valid.and {P Q: vc}:
+  ⊨ P ∧
+  ⊨ Q
+  ↔
+  ⊨ (P && Q)
+
+axiom valid.or {P Q: vc}:
+  (⊨ P ∨ ⊨ Q)
+  ↔
+  ⊨ (P || Q)
+
+axiom valid.mp  {P Q: vc}:
+  (⊨ P → ⊨ Q)
+  ↔
+  ⊨ vc.implies P Q
+
+axiom valid.pre {vₓ: value} {σ: env} {f x y: var} {R S: spec} {e: exp}:
+  ⊨ vc.subst_env (σ[x↦vₓ][f↦value.func f x R S e σ]) R.to_prop.instantiated
+  ↔
+  ⊨ vc.pre (value.func f x R S e σ) vₓ
+
+axiom valid.pre₁ {vₓ v: value} {op: unop}:
+  (∃v, unop.apply op vₓ = some v)
+  ↔
+  ⊨ vc.pre₁ op vₓ
+
+axiom valid.pre₂ {v₁ v₂ v: value} {op: binop}:
+  (∃v, binop.apply op v₁ v₂ = v)
+  ↔
+  ⊨ vc.pre₂ op v₁ v₂
+
+axiom valid.post {vₓ: value} {σ σ': env} {f x y: var} {R S: spec} {e: exp}:
+  (σ[x↦vₓ], e) ⟶* (σ', exp.return y) ∧
+  ⊨ vc.subst_env (σ[x↦vₓ][f↦value.func f x R S e σ]) (spec.implies R S).to_prop.instantiated
+  ↔
+  ⊨ vc.post (value.func f x R S e σ) vₓ
+
+axiom valid.univ {x: var} {P: vc}:
+  (∀v, ⊨ vc.subst x v P)
+  ↔
+  ⊨ vc.univ x P
+
+axiom valid.subst {t₁ t₂: term} (Q: propctx):
+  ⊨ (t₁ ≡ t₂) →
+  ⊨ (Q t₁).instantiated →
+  ⊨ (Q t₂).instantiated
+
+axiom valid.eq.symm {t₁ t₂: term}:
+  ⊨ (t₁ ≡ t₂) →
+  ⊨ (t₂ ≡ t₁)
+
+axiom instantiated_of_erased {P: prop}:
+  ⊨ P.erased →
+  ⊨ P.instantiated
+
+axiom instantiated_n_of_instantiated {P: prop}:
+  ⊨ P.instantiated →
+  ⊨ P.instantiated_n
+
+axiom erased_n_of_instantiated_n {P: prop}:
+  ⊨ P.instantiated_n → ⊨ P.erased_n
+
+axiom instantiated_and {P Q: prop}:
+  ⊨ (P.instantiated && Q.instantiated) → ⊨ (P && Q).instantiated
+
+axiom instantiated_or {P Q: prop}:
+  ⊨ (P.instantiated || Q.instantiated) → ⊨ (P || Q).instantiated
 
 -- lemmas
 
@@ -87,18 +105,30 @@ lemma valid.refl {v: value}: ⊨ (v ≡ v) :=
                                   (classical.prop_decidable (v = v))
                                   value value.true value.false, by unfold binop.apply,
   have binop.apply binop.eq v v = value.true, by simp[this],
-  have h: ⊨ ((v ≡ v) ≡ value.true), from valid.binop this,
-  have ⊨ value.true, from valid.tru,
-  let Q:propctx := propctx.term termctx.hole in
-  show ⊨ (v ≡ v), from valid.subst Q h this
+  have ⊨ ((v ≡ v) ≡ value.true), from valid.binop.mp this,
+  have h: ⊨ (value.true ≡ (v ≡ v)), from valid.eq.symm this,
+  have h2: ⊨ vc.term value.true, from valid.tru,
+  let Q:propctx := propctx.term • in
+  have h3: Q value.true = value.true, by refl,
+  have (prop.term value.true).erased = vc.term value.true, by unfold prop.erased,
+  have (Q value.true).erased = vc.term value.true, from h3 ▸ this,
+  have ⊨ (Q value.true).erased, from this ▸ h2,
+  have ⊨ (Q value.true).instantiated, from instantiated_of_erased this,
+  have ⊨ (Q (v ≡ v)).instantiated, from valid.subst Q h this,
+  have ⊨ (Q (v ≡ v)).instantiated_n, from instantiated_n_of_instantiated this,
+  have h7: ⊨ (Q (v ≡ v)).erased_n, from erased_n_of_instantiated_n this,
+  have Q (v ≡ v) = prop.term (v ≡ v), by refl,
+  have h8: ⊨ (prop.term (v ≡ v)).erased_n, from this ▸ h7,
+  have (prop.term (v ≡ v)).erased = vc.term (v ≡ v), by unfold prop.erased,
+  show ⊨ (v ≡ v), from this ▸ h8
 
 lemma valid_env.and {σ: env} {P Q: vc}: σ ⊨ P → σ ⊨ Q → σ ⊨ (P && Q) :=
-  assume p_valid: valid (vc.subst_env σ P),
-  assume q_valid: valid (vc.subst_env σ Q),
+  assume p_valid: ⊨ vc.subst_env σ P,
+  assume q_valid: ⊨ vc.subst_env σ Q,
   have vc.subst_env σ (P && Q) = (vc.subst_env σ P && vc.subst_env σ Q), from vc.subst_env.and,
-  show σ ⊨ (P && Q), from this.symm ▸ valid.and p_valid q_valid
+  show σ ⊨ (P && Q), from this.symm ▸ valid.and.mp ⟨p_valid, q_valid⟩
 
-lemma valid.mp_env {σ: env} {P Q: vc}: σ ⊨ vc.implies P Q → σ ⊨ P → σ ⊨ Q :=
+lemma valid_env.mp {σ: env} {P Q: vc}: σ ⊨ vc.implies P Q → σ ⊨ P → σ ⊨ Q :=
   assume impl: σ ⊨ (vc.implies P Q),
   assume p: σ ⊨ P,
   have vc.subst_env σ (vc.implies P Q) = (vc.subst_env σ P.not || vc.subst_env σ Q), from vc.subst_env.or,
@@ -106,11 +136,4 @@ lemma valid.mp_env {σ: env} {P Q: vc}: σ ⊨ vc.implies P Q → σ ⊨ P → �
   have vc.subst_env σ P.not = (vc.subst_env σ P).not, from vc.subst_env.not,
   have ⊨ ((vc.subst_env σ P).not || vc.subst_env σ Q), from this ▸ h,
   have ⊨ vc.implies (vc.subst_env σ P) (vc.subst_env σ Q), from this,
-  show σ ⊨ Q, from valid.mp this p
-
-lemma valid.pre₁.inv {vₓ: value} {op: unop}: ⊨ vc.pre₁ op vₓ → (∃v, unop.apply op vₓ = some v) :=
-  assume pre_valid: ⊨ vc.pre₁ op vₓ,
-  show (∃v, unop.apply op vₓ = some v), by begin
-    cases pre_valid,
-    case valid.pre₁ v exist_v { exact exist_v }
-  end
+  show σ ⊨ Q, from valid.mp.mpr this p
