qi.lean
@@ -73,352 +73,257 @@ axiom and_dist_of_no_instantiations {P Q: prop}:
 axiom or_dist_of_no_instantiations {P Q: prop}:
   no_instantiations Q → ((P || Q).instantiated = P.instantiated || Q.erased)
 
-lemma not_free_in_erased_of_not_free {x: var} {P: prop}: x ∉ FV P → (x ∉ FV P.erased ∧ x ∉ FV P.erased_n) :=
-  assume x_not_free_in_P: x ∉ FV P,
+lemma free_of_erased_free {x: var} {P: prop}: (x ∈ FV P.erased ∨ x ∈ FV P.erased_n) → x ∈ FV P :=
+  assume x_free_in_erased_or_erased_n: x ∈ FV P.erased ∨ x ∈ FV P.erased_n,
   begin
     induction P,
     case prop.term t { from (
-      have h1: x ∉ FV t, from (
-        assume : x ∈ FV t,
-        have free_in_prop x (prop.term t), from free_in_prop.term this,
-        show «false», from x_not_free_in_P this
-      ),
-      have h2: (x ∉ FV (prop.term t).erased), from (
+      or.elim x_free_in_erased_or_erased_n
+      (
         assume x_free_in_t: free_in_vc x (prop.term t).erased,
         have (prop.term t).erased = vc.term t, by unfold prop.erased,
         have free_in_vc x (vc.term t), from this ▸ x_free_in_t,
         have free_in_term x t, from free_in_vc.term.inv this,
-        show «false», from h1 this
-      ),
-      have h3: (x ∉ FV (prop.term t).erased_n), from (
+        show free_in_prop x (prop.term t), from free_in_prop.term this
+      ) (
         assume x_free_in_t: free_in_vc x (prop.term t).erased_n,
         have (prop.term t).erased_n = vc.term t, by unfold prop.erased_n,
         have free_in_vc x (vc.term t), from this ▸ x_free_in_t,
         have free_in_term x t, from free_in_vc.term.inv this,
-        show «false», from h1 this
-      ),
-      ⟨h2, h3⟩
+        show free_in_prop x (prop.term t), from free_in_prop.term this
+      )
     )},
     case prop.not P₁ ih { from (
-      have x ∉ FV P₁, from (
-        assume : x ∈ FV P₁,
-        have x ∈ FV P₁.not, from free_in_prop.not this,
-        show «false», from x_not_free_in_P this
-      ),
-      have h1: x ∉ FV P₁.erased, from (ih this).left,
-      have h2: x ∉ FV P₁.erased_n, from (ih this).right,
-      have h3: x ∉ FV (prop.not P₁).erased, from (
+      or.elim x_free_in_erased_or_erased_n
+      (
         assume x_free: x ∈ FV (prop.not P₁).erased,
         have (prop.not P₁).erased = vc.not P₁.erased_n, by unfold prop.erased,
         have x ∈ FV (vc.not P₁.erased_n), from this ▸ x_free,
         have x ∈ FV P₁.erased_n, from free_in_vc.not.inv this,
-        show «false», from h2 this
-      ),
-      have h4: x ∉ FV (prop.not P₁).erased_n, from (
+        have x ∈ FV P₁, from ih (or.inr this),
+        show x ∈ FV P₁.not, from free_in_prop.not this
+      ) (
         assume x_free: x ∈ FV (prop.not P₁).erased_n,
         have (prop.not P₁).erased_n = vc.not P₁.erased, by unfold prop.erased_n,
         have x ∈ FV (vc.not P₁.erased), from this ▸ x_free,
         have x ∈ FV P₁.erased, from free_in_vc.not.inv this,
-        show «false», from h1 this
-      ),
-      ⟨h3, h4⟩
+        have x ∈ FV P₁, from ih (or.inl this),
+        show x ∈ FV P₁.not, from free_in_prop.not this
+      )
     )},
     case prop.and P₁ P₂ P₁_ih P₂_ih { from (
-      have x ∉ FV P₁, from (
-        assume : x ∈ FV P₁,
-        have x ∈ FV (P₁ && P₂), from free_in_prop.and₁ this,
-        show «false», from x_not_free_in_P this
-      ),
-      have h1: x ∉ FV P₁.erased, from (P₁_ih this).left,
-      have h2: x ∉ FV P₁.erased_n, from (P₁_ih this).right,
-      have x ∉ FV P₂, from (
-        assume : x ∈ FV P₂,
-        have x ∈ FV (P₁ && P₂), from free_in_prop.and₂ this,
-        show «false», from x_not_free_in_P this
-      ),
-      have h3: x ∉ FV P₂.erased, from (P₂_ih this).left,
-      have h4: x ∉ FV P₂.erased_n, from (P₂_ih this).right,
-      have h5: x ∉ FV (P₁ && P₂).erased, from (
+      or.elim x_free_in_erased_or_erased_n (
         assume x_free: x ∈ FV (P₁ && P₂).erased,
         have (prop.and P₁ P₂).erased = P₁.erased && P₂.erased, by unfold prop.erased,
         have x ∈ FV (P₁.erased && P₂.erased), from this ▸ x_free,
         have x ∈ FV P₁.erased ∨ x ∈ FV P₂.erased, from free_in_vc.and.inv this,
         or.elim this (
           assume : x ∈ FV P₁.erased,
-          show «false», from h1 this
+          have x ∈ FV P₁, from P₁_ih (or.inl this),
+          show x ∈ FV (P₁ && P₂), from free_in_prop.and₁ this
         ) (
           assume : x ∈ FV P₂.erased,
-          show «false», from h3 this
+          have x ∈ FV P₂, from P₂_ih (or.inl this),
+          show x ∈ FV (P₁ && P₂), from free_in_prop.and₂ this
         )
-      ),
-      have h6: x ∉ FV (P₁ && P₂).erased_n, from (
+      ) (
         assume x_free: x ∈ FV (P₁ && P₂).erased_n,
         have (prop.and P₁ P₂).erased_n = P₁.erased_n && P₂.erased_n, by unfold prop.erased_n,
         have x ∈ FV (P₁.erased_n && P₂.erased_n), from this ▸ x_free,
         have x ∈ FV P₁.erased_n ∨ x ∈ FV P₂.erased_n, from free_in_vc.and.inv this,
         or.elim this (
           assume : x ∈ FV P₁.erased_n,
-          show «false», from h2 this
+          have x ∈ FV P₁, from P₁_ih (or.inr this),
+          show x ∈ FV (P₁ && P₂), from free_in_prop.and₁ this
         ) (
           assume : x ∈ FV P₂.erased_n,
-          show «false», from h4 this
+          have x ∈ FV P₂, from P₂_ih (or.inr this),
+          show x ∈ FV (P₁ && P₂), from free_in_prop.and₂ this
         )
-      ),
-      ⟨h5, h6⟩
+      )
     )},
     case prop.or P₁ P₂ P₁_ih P₂_ih { from (
-      have x ∉ FV P₁, from (
-        assume : x ∈ FV P₁,
-        have x ∈ FV (P₁ || P₂), from free_in_prop.or₁ this,
-        show «false», from x_not_free_in_P this
-      ),
-      have h1: x ∉ FV P₁.erased, from (P₁_ih this).left,
-      have h2: x ∉ FV P₁.erased_n, from (P₁_ih this).right,
-      have x ∉ FV P₂, from (
-        assume : x ∈ FV P₂,
-        have x ∈ FV (P₁ || P₂), from free_in_prop.or₂ this,
-        show «false», from x_not_free_in_P this
-      ),
-      have h3: x ∉ FV P₂.erased, from (P₂_ih this).left,
-      have h4: x ∉ FV P₂.erased_n, from (P₂_ih this).right,
-      have h5: x ∉ FV (P₁ || P₂).erased, from (
+      or.elim x_free_in_erased_or_erased_n (
         assume x_free: x ∈ FV (P₁ || P₂).erased,
         have (prop.or P₁ P₂).erased = P₁.erased || P₂.erased, by unfold prop.erased,
         have x ∈ FV (P₁.erased || P₂.erased), from this ▸ x_free,
         have x ∈ FV P₁.erased ∨ x ∈ FV P₂.erased, from free_in_vc.or.inv this,
         or.elim this (
           assume : x ∈ FV P₁.erased,
-          show «false», from h1 this
+          have x ∈ FV P₁, from P₁_ih (or.inl this),
+          show x ∈ FV (P₁ || P₂), from free_in_prop.or₁ this
         ) (
           assume : x ∈ FV P₂.erased,
-          show «false», from h3 this
+          have x ∈ FV P₂, from P₂_ih (or.inl this),
+          show x ∈ FV (P₁ || P₂), from free_in_prop.or₂ this
         )
-      ),
-      have h6: x ∉ FV (P₁ || P₂).erased_n, from (
+      ) (
         assume x_free: x ∈ FV (P₁ || P₂).erased_n,
         have (prop.or P₁ P₂).erased_n = P₁.erased_n || P₂.erased_n, by unfold prop.erased_n,
         have x ∈ FV (P₁.erased_n || P₂.erased_n), from this ▸ x_free,
         have x ∈ FV P₁.erased_n ∨ x ∈ FV P₂.erased_n, from free_in_vc.or.inv this,
         or.elim this (
           assume : x ∈ FV P₁.erased_n,
-          show «false», from h2 this
+          have x ∈ FV P₁, from P₁_ih (or.inr this),
+          show x ∈ FV (P₁ || P₂), from free_in_prop.or₁ this
         ) (
           assume : x ∈ FV P₂.erased_n,
-          show «false», from h4 this
+          have x ∈ FV P₂, from P₂_ih (or.inr this),
+          show x ∈ FV (P₁ || P₂), from free_in_prop.or₂ this
         )
-      ),
-      ⟨h5, h6⟩
+      )
     )},
     case prop.pre t₁ t₂ { from (
-      have h1: x ∉ FV t₁, from (
-        assume : x ∈ FV t₁,
-        have free_in_prop x (prop.pre t₁ t₂), from free_in_prop.pre₁ this,
-        show «false», from x_not_free_in_P this
-      ),
-      have h2: x ∉ FV t₂, from (
-        assume : x ∈ FV t₂,
-        have free_in_prop x (prop.pre t₁ t₂), from free_in_prop.pre₂ this,
-        show «false», from x_not_free_in_P this
-      ),
-      have h3: x ∉ FV (prop.pre t₁ t₂).erased, from (
+      or.elim x_free_in_erased_or_erased_n (
         assume x_free: x ∈ FV (prop.pre t₁ t₂).erased,
         have (prop.pre t₁ t₂).erased = vc.pre t₁ t₂, by unfold prop.erased,
         have x ∈ FV (vc.pre t₁ t₂), from this ▸ x_free,
         have x ∈ FV t₁ ∨ x ∈ FV t₂, from free_in_vc.pre.inv this,
         or.elim this (
           assume : x ∈ FV t₁,
-          show «false», from h1 this
+          show free_in_prop x (prop.pre t₁ t₂), from free_in_prop.pre₁ this
         ) (
           assume : x ∈ FV t₂,
-          show «false», from h2 this
+          show free_in_prop x (prop.pre t₁ t₂), from free_in_prop.pre₂ this
         )
-      ),
-      have h4: x ∉ FV (prop.pre t₁ t₂).erased_n, from (
+      ) (
         assume x_free: x ∈ FV (prop.pre t₁ t₂).erased_n,
         have (prop.pre t₁ t₂).erased_n = vc.pre t₁ t₂, by unfold prop.erased_n,
         have x ∈ FV (vc.pre t₁ t₂), from this ▸ x_free,
         have x ∈ FV t₁ ∨ x ∈ FV t₂, from free_in_vc.pre.inv this,
         or.elim this (
           assume : x ∈ FV t₁,
-          show «false», from h1 this
+          show free_in_prop x (prop.pre t₁ t₂), from free_in_prop.pre₁ this
         ) (
           assume : x ∈ FV t₂,
-          show «false», from h2 this
+          show free_in_prop x (prop.pre t₁ t₂), from free_in_prop.pre₂ this
         )
-      ),
-      ⟨h3, h4⟩
+      )
     )},
     case prop.pre₁ op t { from (
-      have h1: x ∉ FV t, from (
-        assume : x ∈ FV t,
-        have free_in_prop x (prop.pre₁ op t), from free_in_prop.preop this,
-        show «false», from x_not_free_in_P this
-      ),
-      have h2: (x ∉ FV (prop.pre₁ op t).erased), from (
+      or.elim x_free_in_erased_or_erased_n (
         assume x_free_in_t: free_in_vc x (prop.pre₁ op t).erased,
         have (prop.pre₁ op t).erased = vc.pre₁ op t, by unfold prop.erased,
         have free_in_vc x (vc.pre₁ op t), from this ▸ x_free_in_t,
         have free_in_term x t, from free_in_vc.pre₁.inv this,
-        show «false», from h1 this
-      ),
-      have h3: (x ∉ FV (prop.pre₁ op t).erased_n), from (
+        show free_in_prop x (prop.pre₁ op t), from free_in_prop.preop this
+      ) (
         assume x_free_in_t: free_in_vc x (prop.pre₁ op t).erased_n,
         have (prop.pre₁ op t).erased_n = vc.pre₁ op t, by unfold prop.erased_n,
         have free_in_vc x (vc.pre₁ op t), from this ▸ x_free_in_t,
         have free_in_term x t, from free_in_vc.pre₁.inv this,
-        show «false», from h1 this
-      ),
-      ⟨h2, h3⟩
+        show free_in_prop x (prop.pre₁ op t), from free_in_prop.preop this
+      )
     )},
     case prop.pre₂ op t₁ t₂ { from (
-      have h1: x ∉ FV t₁, from (
-        assume : x ∈ FV t₁,
-        have free_in_prop x (prop.pre₂ op t₁ t₂), from free_in_prop.preop₁ this,
-        show «false», from x_not_free_in_P this
-      ),
-      have h2: x ∉ FV t₂, from (
-        assume : x ∈ FV t₂,
-        have free_in_prop x (prop.pre₂ op t₁ t₂), from free_in_prop.preop₂ this,
-        show «false», from x_not_free_in_P this
-      ),
-      have h3: x ∉ FV (prop.pre₂ op t₁ t₂).erased, from (
+      or.elim x_free_in_erased_or_erased_n (
         assume x_free: x ∈ FV (prop.pre₂ op t₁ t₂).erased,
         have (prop.pre₂ op t₁ t₂).erased = vc.pre₂ op t₁ t₂, by unfold prop.erased,
         have x ∈ FV (vc.pre₂ op t₁ t₂), from this ▸ x_free,
         have x ∈ FV t₁ ∨ x ∈ FV t₂, from free_in_vc.pre₂.inv this,
         or.elim this (
           assume : x ∈ FV t₁,
-          show «false», from h1 this
+          show free_in_prop x (prop.pre₂ op t₁ t₂), from free_in_prop.preop₁ this
         ) (
           assume : x ∈ FV t₂,
-          show «false», from h2 this
+          show free_in_prop x (prop.pre₂ op t₁ t₂), from free_in_prop.preop₂ this
         )
-      ),
-      have h4: x ∉ FV (prop.pre₂ op t₁ t₂).erased_n, from (
+      ) (
         assume x_free: x ∈ FV (prop.pre₂ op t₁ t₂).erased_n,
         have (prop.pre₂ op t₁ t₂).erased_n = vc.pre₂ op t₁ t₂, by unfold prop.erased_n,
         have x ∈ FV (vc.pre₂ op t₁ t₂), from this ▸ x_free,
         have x ∈ FV t₁ ∨ x ∈ FV t₂, from free_in_vc.pre₂.inv this,
         or.elim this (
           assume : x ∈ FV t₁,
-          show «false», from h1 this
+          show free_in_prop x (prop.pre₂ op t₁ t₂), from free_in_prop.preop₁ this
         ) (
           assume : x ∈ FV t₂,
-          show «false», from h2 this
+          show free_in_prop x (prop.pre₂ op t₁ t₂), from free_in_prop.preop₂ this
         )
-      ),
-      ⟨h3, h4⟩
+      )
     )},
     case prop.post t₁ t₂ { from (
-      have h1: x ∉ FV t₁, from (
-        assume : x ∈ FV t₁,
-        have free_in_prop x (prop.post t₁ t₂), from free_in_prop.post₁ this,
-        show «false», from x_not_free_in_P this
-      ),
-      have h2: x ∉ FV t₂, from (
-        assume : x ∈ FV t₂,
-        have free_in_prop x (prop.post t₁ t₂), from free_in_prop.post₂ this,
-        show «false», from x_not_free_in_P this
-      ),
-      have h3: x ∉ FV (prop.post t₁ t₂).erased, from (
+      or.elim x_free_in_erased_or_erased_n (
         assume x_free: x ∈ FV (prop.post t₁ t₂).erased,
         have (prop.post t₁ t₂).erased = vc.post t₁ t₂, by unfold prop.erased,
         have x ∈ FV (vc.post t₁ t₂), from this ▸ x_free,
         have x ∈ FV t₁ ∨ x ∈ FV t₂, from free_in_vc.post.inv this,
         or.elim this (
           assume : x ∈ FV t₁,
-          show «false», from h1 this
+
+          show free_in_prop x (prop.post t₁ t₂), from free_in_prop.post₁ this
         ) (
           assume : x ∈ FV t₂,
-          show «false», from h2 this
+
+          show free_in_prop x (prop.post t₁ t₂), from free_in_prop.post₂ this
         )
-      ),
-      have h4: x ∉ FV (prop.post t₁ t₂).erased_n, from (
+      ) (
         assume x_free: x ∈ FV (prop.post t₁ t₂).erased_n,
         have (prop.post t₁ t₂).erased_n = vc.post t₁ t₂, by unfold prop.erased_n,
         have x ∈ FV (vc.post t₁ t₂), from this ▸ x_free,
         have x ∈ FV t₁ ∨ x ∈ FV t₂, from free_in_vc.post.inv this,
         or.elim this (
           assume : x ∈ FV t₁,
-          show «false», from h1 this
+
+          show free_in_prop x (prop.post t₁ t₂), from free_in_prop.post₁ this
         ) (
           assume : x ∈ FV t₂,
-          show «false», from h2 this
+
+          show free_in_prop x (prop.post t₁ t₂), from free_in_prop.post₂ this
         )
-      ),
-      ⟨h3, h4⟩
+      )
     )},
     case prop.call t₁ t₂ { from (
-      have h1: x ∉ FV (prop.call t₁ t₂).erased, from (
+      or.elim x_free_in_erased_or_erased_n (
         assume x_free: x ∈ FV (prop.call t₁ t₂).erased,
         have (prop.call t₁ t₂).erased = vc.term value.true, by unfold prop.erased,
         have x ∈ FV (vc.term value.true), from this ▸ x_free,
         have x ∈ FV (term.value value.true), from free_in_vc.term.inv this,
-        show «false», from (free_in_term.value.inv) this
-      ),
-      have h2: x ∉ FV (prop.call t₁ t₂).erased_n, from (
+        absurd this (free_in_term.value.inv)
+      ) (
         assume x_free: x ∈ FV (prop.call t₁ t₂).erased_n,
         have (prop.call t₁ t₂).erased_n = vc.term value.true, by unfold prop.erased_n,
         have x ∈ FV (vc.term value.true), from this ▸ x_free,
         have x ∈ FV (term.value value.true), from free_in_vc.term.inv this,
-        show «false», from (free_in_term.value.inv) this
-      ),
-      ⟨h1, h2⟩
+        absurd this (free_in_term.value.inv)
+      )
     )},
     case prop.forallc y t P₁ ih { from (
-      have h1: x ∉ FV (prop.forallc y t P₁).erased, from (
+      or.elim x_free_in_erased_or_erased_n (
         assume x_free: x ∈ FV (prop.forallc y t P₁).erased,
         have (prop.forallc y t P₁).erased = vc.univ y P₁.erased, by unfold prop.erased,
         have x ∈ FV (vc.univ y P₁.erased), from this ▸ x_free,
         have h2: (x ≠ y) ∧ free_in_vc x P₁.erased, from free_in_vc.univ.inv this,
-        have x ∉ FV P₁, from (
-          assume : x ∈ FV P₁,
-          have x ∈ FV (prop.forallc y t P₁), from free_in_prop.forallc₂ h2.left this,
-          show «false», from x_not_free_in_P this
-        ),
-        have x ∉ FV P₁.erased, from (ih this).left,
-        show «false», from this h2.right
-      ),
-      have h3: x ∉ FV (prop.forallc y t P₁).erased_n, from (
+        have x ∈ FV P₁, from ih (or.inl h2.right),
+        show x ∈ FV (prop.forallc y t P₁), from free_in_prop.forallc₂ h2.left this
+      ) (
         assume x_free: x ∈ FV (prop.forallc y t P₁).erased_n,
         have (prop.forallc y t P₁).erased_n = vc.term value.true, by unfold prop.erased_n,
         have x ∈ FV (vc.term value.true), from this ▸ x_free,
         have x ∈ FV (term.value value.true), from free_in_vc.term.inv this,
-        show «false», from (free_in_term.value.inv) this
-      ),
-      ⟨h1, h3⟩
+        absurd this (free_in_term.value.inv)
+      )
     )},
     case prop.exis y P₁ ih { from (
-      have h1: x ∉ FV (prop.exis y P₁).erased, from (
+      or.elim x_free_in_erased_or_erased_n (
         assume x_free: x ∈ FV (prop.exis y P₁).erased,
         have (prop.exis y P₁).erased = vc.not (vc.univ y (vc.not P₁.erased)), by unfold prop.erased,
         have x ∈ FV (vc.not (vc.univ y (vc.not P₁.erased))), from this ▸ x_free,
         have x ∈ FV (vc.univ y (vc.not P₁.erased)), from free_in_vc.not.inv this,
         have h2: (x ≠ y) ∧ free_in_vc x (vc.not P₁.erased), from free_in_vc.univ.inv this,
         have h3: x ∈ FV P₁.erased, from free_in_vc.not.inv h2.right,
-        have x ∉ FV P₁, from (
-          assume : x ∈ FV P₁,
-          have x ∈ FV (prop.exis y P₁), from free_in_prop.exis h2.left this,
-          show «false», from x_not_free_in_P this
-        ),
-        have x ∉ FV P₁.erased, from (ih this).left,
-        show «false», from this h3
-      ),
-      have h4: x ∉ FV (prop.exis y P₁).erased_n, from (
+        have x ∈ FV P₁, from ih (or.inl h3),
+        show x ∈ FV (prop.exis y P₁), from free_in_prop.exis h2.left this
+      )
+      (
         assume x_free: x ∈ FV (prop.exis y P₁).erased_n,
         have (prop.exis y P₁).erased_n = vc.not (vc.univ y (vc.not P₁.erased_n)), by unfold prop.erased_n,
         have x ∈ FV (vc.not (vc.univ y (vc.not P₁.erased_n))), from this ▸ x_free,
         have x ∈ FV (vc.univ y (vc.not P₁.erased_n)), from free_in_vc.not.inv this,
-        have h5: (x ≠ y) ∧ free_in_vc x (vc.not P₁.erased_n), from free_in_vc.univ.inv this,
-        have h6: x ∈ FV P₁.erased_n, from free_in_vc.not.inv h5.right,
-        have x ∉ FV P₁, from (
-          assume : x ∈ FV P₁,
-          have x ∈ FV (prop.exis y P₁), from free_in_prop.exis h5.left this,
-          show «false», from x_not_free_in_P this
-        ),
-        have x ∉ FV P₁.erased_n, from (ih this).right,
-        show «false», from this h6
-      ),
-      ⟨h1, h4⟩
+        have h2: (x ≠ y) ∧ free_in_vc x (vc.not P₁.erased_n), from free_in_vc.univ.inv this,
+        have h3: x ∈ FV P₁.erased_n, from free_in_vc.not.inv h2.right,
+        have x ∈ FV P₁, from ih (or.inr h3),
+        show x ∈ FV (prop.exis y P₁), from free_in_prop.exis h2.left this
+      )
     )}
   end
